wip

fstar/api/MLS.API.High.fst
@@ -7,6 +7,11 @@ open MLS.Crypto
 open MLS.NetworkTypes
 open MLS.TreeSync.NetworkTypes
 open MLS.TreeKEM.NetworkTypes
+open MLS.TreeDEM.NetworkTypes
+open MLS.TreeDEM.Welcome
+open MLS.TreeSync.Invariants.AuthService
+
+#set-options "--fuel 0 --ifuel 0"
 
 class entropy (bytes:Type0) (t:Type) = {
   rel: t -> t -> prop;
@@ -40,6 +45,7 @@ let (let*) #bytes #entropy_t #entropy_tc #a #b x f e0 =
   rel_trans #bytes e0 e1 e2;
   (e2, y_value)
 
+#push-options "--ifuel 1"
 val (let*?):
   #bytes:Type0 -> #entropy_t:Type -> {|entropy bytes entropy_t|} ->
   #a:Type -> #b:Type ->
@@ -54,6 +60,7 @@ let (let*?) #bytes #entropy_t #entropy_tc #a #b x f e0 =
   )
   | InternalError s -> (e1, InternalError s)
   | ProtocolError s -> (e1, ProtocolError s)
+#pop-options
 
 val extract_entropy:  
   #bytes:Type0 -> {|bytes_like bytes|} -> #entropy_t:Type -> {|entropy bytes entropy_t|} ->
@@ -71,27 +78,38 @@ let gen_sign_nonce #bytes #cb #entropy_t #entropy_tc =
   let* res = extract_entropy #bytes #_ #entropy_t (sign_sign_min_entropy_length #bytes) in
   return_prob (res <: sign_nonce bytes)
 
-type mls_group = {
+noeq
+type mls_group (bytes:Type0) {|crypto_bytes bytes|} (asp:as_parameters bytes) = {
+  group_id: mls_bytes bytes;
   epoch: nat_lbytes 8;
+  my_leaf_index: nat;
+  my_signature_key: bytes;
+  treesync: MLS.TreeSync.API.Types.treesync_state bytes tkt asp group_id;
+  treekem: MLS.TreeKEM.API.Types.treekem_state bytes my_leaf_index;
 }
 
-type unvalidated_proposal
-type validated_proposal
-type unvalidated_commit
-type validated_commit
+assume new type unvalidated_proposal
+assume new type validated_proposal
+assume new type unvalidated_commit
+assume new type validated_commit
 
 type credential (bytes:Type0) {|bytes_like bytes|} = {
   cred: credential_nt bytes;
-  signature_public_key: bytes;
+  signature_public_key: signature_public_key_nt bytes;
 }
 
-type credential_pair (bytes:Type0) {|bytes_like bytes|} = {
+type token_for (#bytes:Type0) {|bytes_like bytes|} (asp:as_parameters bytes) (vk:signature_public_key_nt bytes) (cred:credential_nt bytes) =
+  tok:asp.token_t{asp.credential_ok (vk, cred) tok}
+
+noeq
+type credential_pair (bytes:Type0) {|bytes_like bytes|} (asp:as_parameters bytes) = {
   cred: credential bytes;
   signature_private_key: bytes;
+  token: token_for asp cred.signature_public_key cred.cred;
 }
 
 type signature_keypair (bytes:Type0) {|bytes_like bytes|} = {
-  public_key: bytes;
+  public_key: signature_public_key_nt bytes;
   private_key: bytes;
 }
 
@@ -138,6 +156,7 @@ val generate_signature_keypair:
 let generate_signature_keypair #bytes #cb #entropy_t #entropy_tc =
   let* rand = extract_entropy (sign_gen_keypair_min_entropy_length #bytes) in
   let*? (vk, sk) = return_prob (sign_gen_keypair rand) in
+  let*? vk = return_prob (mk_mls_bytes vk "generate_signature_keypair" "vk") in
   return_prob #bytes #entropy_t (return ({
     public_key = vk;
     private_key = sk;
@@ -146,45 +165,30 @@ let generate_signature_keypair #bytes #cb #entropy_t #entropy_tc =
 val get_signature_public_key:
   #bytes:Type0 -> {|bytes_like bytes|} ->
   signature_keypair bytes ->
-  bytes
+  signature_public_key_nt bytes
 let get_signature_public_key #bytes #bl sig_kp =
   sig_kp.public_key
 
-val mk_credential_:
+val mk_credential:
   #bytes:Type0 -> {|bytes_like bytes|} ->
-  signature_keypair bytes -> credential_nt bytes ->
-  credential_pair bytes
-let mk_credential_ #bytes #bl sig_keypair cred =
+  #asp:as_parameters bytes ->
+  sig_keypair:signature_keypair bytes -> cred:credential_nt bytes ->
+  token_for asp (get_signature_public_key sig_keypair) cred ->
+  credential_pair bytes asp
+let mk_credential #bytes #bl #asp sig_keypair cred token =
   {
     cred = {
       cred;
       signature_public_key = sig_keypair.public_key;
     };
     signature_private_key = sig_keypair.private_key;
+    token;
   }
-
-val mk_basic_credential:
-  #bytes:Type0 -> {|bytes_like bytes|} ->
-  signature_keypair bytes -> identity:bytes ->
-  result (credential_pair bytes)
-let mk_basic_credential #bytes #bl sig_keypair identity =
-  let? identity = mk_mls_bytes identity "mk_basic_credential" "identity" in
-  let cred = C_basic identity in
-  return (mk_credential_ sig_keypair cred)
-
-val mk_x509_credential:
-  #bytes:Type0 -> {|bytes_like bytes|} ->
-  signature_keypair bytes -> x509_chain:list bytes ->
-  result (credential_pair bytes)
-let mk_x509_credential #bytes #bl sig_keypair x509_chain =
-  let? chain = mapM (fun x -> mk_mls_bytes x "mk_x509_credential" "cert_data") x509_chain in
-  let? chain = mk_mls_list chain "mk_x509_credential" "chain" in
-  let cred = C_x509 chain in
-  return (mk_credential_ sig_keypair cred)
 
 val get_public_credential:
   #bytes:Type0 -> {|bytes_like bytes|} ->
-  credential_pair bytes ->
+  #asp:as_parameters bytes ->
+  credential_pair bytes asp ->
   credential bytes
 let get_public_credential #bytes #bl cred_pair =
   cred_pair.cred
@@ -212,14 +216,13 @@ val create_leaf_node_data_:
   #bytes:Type0 -> {|crypto_bytes bytes|} ->
   #entropy_t:Type0 -> {|entropy bytes entropy_t|} ->
   credential bytes ->
-  prob #bytes #entropy_t (result (leaf_node_data_nt bytes tkt & bytes))
+  prob #bytes #entropy_t (result (leaf_node_data_nt bytes tkt & hpke_private_key bytes))
 let create_leaf_node_data_ #bytes #cb #entropy_t #entropy_tc cred =
   let* rand = extract_entropy (hpke_private_key_length #bytes) in
   let*? (decryption_key, encryption_key) = return_prob (hpke_gen_keypair rand) in
   let*? encryption_key = return_prob (mk_mls_bytes ((encryption_key <: lbytes bytes (hpke_public_key_length #bytes)) <: bytes) "" "") in
   let*? capabilities = return_prob default_capabilities_ in
   let extensions = MLS.TreeSync.Extensions.empty_extensions #bytes #cb.base in
-  assume(length cred.signature_public_key < pow2 30);
   cb.hpke_public_key_length_bound;
   let leaf_node_data: leaf_node_data_nt bytes tkt = {
     content = encryption_key;
@@ -231,14 +234,15 @@ let create_leaf_node_data_ #bytes #cb #entropy_t #entropy_tc cred =
     parent_hash = ();
     extensions;
   } in
-  return_prob (return (leaf_node_data, ((decryption_key <: lbytes bytes (hpke_private_key_length #bytes)) <: bytes)))
+  return_prob (return (leaf_node_data, decryption_key))
 
 val create_leaf_node_:
   #bytes:Type0 -> {|crypto_bytes bytes|} ->
   #entropy_t:Type0 -> {|entropy bytes entropy_t|} ->
-  credential_pair bytes ->
-  prob #bytes #entropy_t (result (leaf_node_nt bytes tkt & bytes))
-let create_leaf_node_ #bytes #cb #entropy_t #entropy_tc cred_pair =
+  #asp:as_parameters bytes ->
+  credential_pair bytes asp ->
+  prob #bytes #entropy_t (result (leaf_node_nt bytes tkt & hpke_private_key bytes))
+let create_leaf_node_ #bytes #cb #entropy_t #entropy_tc #asp cred_pair =
   let*? (leaf_node_data, decryption_key) = create_leaf_node_data_ cred_pair.cred in
   let* nonce = gen_sign_nonce in
   assume(leaf_node_data.source == LNS_key_package);
@@ -246,6 +250,7 @@ let create_leaf_node_ #bytes #cb #entropy_t #entropy_tc cred_pair =
   return_prob (return (leaf_node, decryption_key))
 
 type keystore_value_type (bytes:Type0) {|bytes_like bytes|} = {
+  key_package: key_package_nt bytes tkt;
   leaf_node_decryption_key: bytes;
   key_package_decryption_key: bytes;
   signature_private_key: bytes;
@@ -258,12 +263,14 @@ type create_key_package_result (bytes:Type0) {|bytes_like bytes|} = {
   keystore_value: keystore_value_type bytes;
 }
 
+#push-options "--ifuel 1 --fuel 1"
 val create_key_package_:
   #bytes:Type0 -> {|crypto_bytes bytes|} ->
   #entropy_t:Type0 -> {|entropy bytes entropy_t|} ->
-  credential_pair bytes ->
-  prob #bytes #entropy_t (result (key_package_nt bytes tkt & keystore_value_type bytes))
-let create_key_package_ #bytes #cb #entropy_t #entropy_tc cred_pair =
+  #asp:as_parameters bytes ->
+  credential_pair bytes asp ->
+  prob #bytes #entropy_t (result (keystore_value_type bytes))
+let create_key_package_ #bytes #cb #entropy_t #entropy_tc #asp cred_pair =
   let*? (leaf_node, leaf_node_decryption_key) = create_leaf_node_ cred_pair in
   let* rand = extract_entropy (hpke_private_key_length #bytes) in
   let*? (key_package_decryption_key, init_key) = return_prob (hpke_gen_keypair rand) in
@@ -281,24 +288,27 @@ let create_key_package_ #bytes #cb #entropy_t #entropy_tc cred_pair =
   let tbs: bytes = (ps_prefix_to_ps_whole (ps_key_package_tbs_nt _)).serialize kp_tbs in
   let*? signature: bytes = return_prob (sign_with_label cred_pair.signature_private_key "KeyPackageTBS" tbs nonce) in
   let*? signature = return_prob (mk_mls_bytes signature "create_key_package_" "signature") in
-  let key_package = {
+  let key_package: key_package_nt bytes tkt = {
     tbs = kp_tbs;
     signature;
   } in
-  let keystore_value = {
+  return_prob (return ({
+    key_package;
     leaf_node_decryption_key;
     key_package_decryption_key;
     signature_private_key = cred_pair.signature_private_key;
-  } in
-  return_prob (return (key_package, keystore_value))
+  } <: keystore_value_type bytes))
+#pop-options
 
 val create_key_package:
   #bytes:Type0 -> {|crypto_bytes bytes|} ->
   #entropy_t:Type0 -> {|entropy bytes entropy_t|} ->
-  credential_pair bytes ->
+  #asp:as_parameters bytes ->
+  credential_pair bytes asp ->
   prob #bytes #entropy_t (result (create_key_package_result bytes))
-let create_key_package #bytes #cb #entropy_t #entropy_tc cred_pair =
-  let*? key_package, keystore_value = create_key_package_ cred_pair in
+let create_key_package #bytes #cb #entropy_t #entropy_tc #asp cred_pair =
+  let*? keystore_value = create_key_package_ cred_pair in
+  let key_package = keystore_value.key_package in
   let key_package_bytes = (ps_prefix_to_ps_whole (ps_key_package_nt _)).serialize key_package in
   let*? keystore_key = return_prob (MLS.TreeDEM.KeyPackageRef.compute_key_package_ref key_package) in
   let keystore_key = ((keystore_key <: MLS.TreeDEM.NetworkTypes.key_package_ref_nt bytes) <: bytes) in
@@ -310,21 +320,165 @@ let create_key_package #bytes #cb #entropy_t #entropy_tc cred_pair =
 
 (*** Group creation ***)
 
-val create_group:
-  #bytes:Type0 -> {|bytes_like bytes|} ->
+val create_group_with_group_id:
+  #bytes:Type0 -> {|crypto_bytes bytes|} ->
   #entropy_t:Type0 -> {|entropy bytes entropy_t|} ->
-  entropy_t ->
-  credential_pair bytes ->
-  entropy_t & (result mls_group)
+  #asp:as_parameters bytes ->
+  credential_pair bytes asp -> bytes ->
+  prob #bytes #entropy_t (result (mls_group bytes asp))
+let create_group_with_group_id #bytes #bl #entropy_t #entropy_tc #asp cred_pair group_id =
+  let*? group_id = return_prob (mk_mls_bytes group_id "create_group_with_group_id" "group_id") in
+  let*? (my_leaf_node, my_decryption_key) = create_leaf_node_ cred_pair in
+  let*? pending_treesync = return_prob (MLS.TreeSync.API.prepare_create group_id my_leaf_node) in
+  assume(my_leaf_node.data.signature_key == cred_pair.cred.signature_public_key);
+  assume(my_leaf_node.data.credential == cred_pair.cred.cred);
+  let treesync = MLS.TreeSync.API.finalize_create pending_treesync cred_pair.token in
+  let* epoch_secret = extract_entropy (kdf_length #bytes) in
+  let*? (treekem, encryption_secret) = return_prob (MLS.TreeKEM.API.create my_decryption_key (my_leaf_node.data.content <: bytes) epoch_secret) in
+  //TODO TreeDEM state
+  return_prob (return ({
+    group_id;
+    epoch = 0;
+    my_leaf_index = 0;
+    my_signature_key = cred_pair.signature_private_key;
+    treesync;
+    treekem;
+  } <: mls_group bytes asp))
+
+val create_group:
+  #bytes:Type0 -> {|crypto_bytes bytes|} ->
+  #entropy_t:Type0 -> {|entropy bytes entropy_t|} ->
+  #asp:as_parameters bytes ->
+  credential_pair bytes asp ->
+  prob #bytes #entropy_t (result (mls_group bytes asp))
+let create_group #bytes #cb #entropy_t #entropy_tc #asp cred_pair =
+  let* group_id = extract_entropy (kdf_length #bytes) in
+  create_group_with_group_id cred_pair group_id
 
 let key_lookup (bytes:Type0) {|bytes_like bytes|} = bytes -> option (keystore_value_type bytes)
-val join_group:
-  #bytes:Type0 -> {|bytes_like bytes|} ->
-  welcome:bytes ->
-  key_lookup bytes ->
-  result mls_group
 
-val join_with_external_commit:
-  unit -> //TODO
-  result mls_group
+type start_join_group_output (bytes:Type0) {|bytes_like bytes|} = {
+  group_info: group_info_nt bytes;
+  group_secrets: group_secrets_nt bytes;
+  my_kp_ref: bytes;
+  my_kp_store_value: keystore_value_type bytes;
+}
+
+val start_join_group:
+  #bytes:Type0 -> {|crypto_bytes bytes|} ->
+  welcome:welcome_nt bytes ->
+  key_lookup bytes ->
+  result (start_join_group_output bytes)
+let start_join_group #bytes #cb w lookup =
+  let extract_hpke_sk (keystore_value:keystore_value_type bytes): result (hpke_private_key bytes) =
+    let res = keystore_value.key_package_decryption_key in
+    if not (length res = hpke_private_key_length #bytes) then
+      error ""
+    else
+      return res
+  in
+  let? (group_info, group_secrets, (my_kp_ref, my_kp_store_value)) =
+    (MLS.TreeDEM.Welcome.decrypt_welcome w lookup extract_hpke_sk)
+  in
+  return ({
+    group_info;
+    group_secrets;
+    my_kp_ref;
+    my_kp_store_value;
+  })
+
+// TODO: getters for start_join_group_output
+// - group_id / tree_hash (or simply group_context?)
+// - ratchet_tree
+
+#push-options "--fuel 0 --ifuel 1"
+type continue_join_group_output (bytes:Type0) {|crypto_bytes bytes|} = {
+  step_before: start_join_group_output bytes;
+  l: nat;
+  treesync: MLS.TreeSync.Types.treesync bytes tkt l 0;
+  welcome_pend: MLS.TreeSync.API.pending_welcome step_before.group_info.tbs.group_context.group_id treesync;
+}
+#pop-options
+
+#push-options "--fuel 0 --ifuel 1"
+val continue_join_group:
+  #bytes:Type0 -> {|crypto_bytes bytes|} ->
+  start_join_group_output bytes -> option (ratchet_tree_nt bytes tkt) ->
+  result (continue_join_group_output bytes)
+let continue_join_group #bytes #cb step_before opt_ratchet_tree =
+  let? ratchet_tree =
+    match opt_ratchet_tree with
+    | Some ratchet_tree -> return ratchet_tree
+    | None -> (
+      //TODO: look in the group_info extensions
+      internal_failure ""
+    )
+  in
+  let? (|l, treesync|) = MLS.NetworkBinder.ratchet_tree_to_treesync ratchet_tree in
+  let? welcome_pend = MLS.TreeSync.API.prepare_welcome step_before.group_info.tbs.group_context.group_id treesync in
+  return ({
+    step_before;
+    l;
+    treesync;
+    welcome_pend;
+  })
+#pop-options
+
+val find_my_index:
+  #bytes:eqtype -> {|bytes_like bytes|} ->
+  #l:nat -> MLS.TreeSync.Types.treesync bytes tkt l 0 -> leaf_node_nt bytes tkt ->
+  result (res:nat{res<pow2 l})
+let find_my_index #bytes #bl #l t ln =
+  let test (oln: option (leaf_node_nt bytes tkt)) =
+    oln = Some ln
+  in
+  from_option "find_my_index: can't find my_index" (MLS.Utils.find_first test (MLS.Tree.get_leaf_list t))
+
+val finalize_join_group:
+  #bytes:Type0 -> {|crypto_bytes bytes|} ->
+  #asp:as_parameters bytes ->
+  step_before:continue_join_group_output bytes -> MLS.TreeSync.API.tokens_for_welcome asp step_before.welcome_pend ->
+  result (mls_group bytes asp)
+let finalize_join_group #bytes #cb #asp step_before tokens =
+  //TODO handle PSK somewhere
+  bytes_hasEq #bytes;
+  let my_kp_store_value = step_before.step_before.my_kp_store_value in
+  let my_leaf_node = my_kp_store_value.key_package.tbs.leaf_node in
+  let treesync_state = MLS.TreeSync.API.finalize_welcome step_before.welcome_pend tokens in
+
+  // TODO check group info
+  // - check signature
+  // - check ciphersuite compared to keypackage
+  // - check tree hash is the same as ratchet tree
+  // - stuff with confirmation tag and transcript hash?
+
+  let? my_leaf_index = find_my_index step_before.treesync my_leaf_node in
+
+  let? treekem = MLS.TreeSyncTreeKEMBinder.treesync_to_treekem step_before.treesync in
+  assume(Some? (MLS.Tree.leaf_at treekem my_leaf_index)); // Can be proved
+  assume(MLS.TreeKEM.Invariants.treekem_invariant treekem); // Can be proved
+  let opt_path_secret_and_inviter_ind: option (bytes & nat) = match step_before.step_before.group_secrets.path_secret with | None -> None | Some {path_secret} -> Some (path_secret, step_before.step_before.group_info.tbs.signer) in
+  let group_context = step_before.step_before.group_info.tbs.group_context in
+  let leaf_decryption_key = my_kp_store_value.leaf_node_decryption_key in
+  assume(length leaf_decryption_key == hpke_private_key_length #bytes);
+  let? epoch_secret = MLS.TreeKEM.KeySchedule.secret_joiner_to_epoch step_before.step_before.group_secrets.joiner_secret None ((ps_prefix_to_ps_whole ps_group_context_nt).serialize group_context) in
+  let? (treekem_state, encryption_secret) = MLS.TreeKEM.API.welcome treekem leaf_decryption_key opt_path_secret_and_inviter_ind my_leaf_index epoch_secret in
+
+  // TODO TreeDEM
+
+  return ({
+    group_id = step_before.step_before.group_info.tbs.group_context.group_id;
+    epoch = step_before.step_before.group_info.tbs.group_context.epoch;
+    my_leaf_index;
+    my_signature_key = my_kp_store_value.signature_private_key;
+    treesync = treesync_state;
+    treekem = treekem_state;
+  } <: mls_group bytes asp)
+
+
+
+
+//val join_with_external_commit:
+//  unit -> //TODO
+//  result mls_group
 
